cesm_im.v
@@ -1,49 +1,205 @@
 Require Import util cesm im db db_assembly assembly relations List cem.
 Import ListNotations.
+Require Import Program.
 
 Open Scope nat_scope. 
-Variable new : ∀ (n:nat) (h : im.Heap), sigT (λ w:nat, ∀ i, lt i n → (i+w) ∉ domain h).
+(*
+Variable new : ∀ (n:nat) (h : im.Heap), sigT (λ w:nat, 
+  prod (∀ i, lt i n → (i+w) ∉ domain h)
+       (w > 0)).
+*)
 
 Definition prog_eq (p : Ptr) (pr : Program) (t : tm) := 
   let subpr := assemble t p in subpr = firstn (length subpr) (skipn p pr).
 
+(*
 Inductive env_eq : nat → cem.heap → 
                    Program → Ptr → im.Heap → Type := 
   | ee : ∀ n ch pr p ih e e' c c' ip t, 
-    lookup n ch = Some (cl (close t e) c) →
-    lookup p ih = Some ip → 
-    lookup (1+p) ih = Some e' → 
-    lookup (2+p) ih = Some c' → 
+    (lookup n ch = Some (cl (close t e) c) →
+    (prod (lookup p ih = Some ip)  
+    (prod (lookup (1+p) ih = Some e')
+    (lookup (2+p) ih = Some c')))) → 
     prog_eq ip pr t → 
     env_eq e ch pr e' ih →    
     env_eq c ch pr c' ih →    
     env_eq n ch pr p ih.
+*)  
+(*
+Inductive heap_eq : (nat, cell) → (Ptr * Ptr * Ptr * Ptr), P → cem.heap → im.heap → Type :=
+  | heap_eq_tail : ∀ l p, (l, 
+*)
+
+Inductive heap_rel : cesm.heap → im.Heap → Type := 
+  | heap_nil : heap_rel [] [] 
+  | heap_cons : ∀ l l' ne ch ih ip ep ine e t, 
+    l ∉ domain ch → l' ∉ domain ih → S l' ∉ domain ih → S (S l') ∉ domain ih →
+    l > 0 → l' > 0 → 
+    heap_rel ch ih → 
+    heap_rel 
+      ((l, cl (close t e) ne)::ch) 
+      ((l', ip)::(S l', ep)::(S (S l'), ine)::ih).
+
+(*
+Inductive in_heap : ∀ (ch : cesm.heap) (ih : im.Heap) (r : heap_rel ch ih) 
+  (l e ne : nat) (t : db.tm) (il ip ep nep : Ptr), Type :=
+  | in_heap_head : in_heap_rel ((l, cl (close t e) ne)::ch)
+                               ((il, ip)::(S il, ep)::(S (S il), ine)::ih)
+  | in_heap_tail : in_heap_rel ch ih r l e ne t il ip ep nep →
+                   in_heap_rel ((l', cl (close t' e') ne')::ch) 
+                               ((il', ip)::(S il', ep)::(S (S il'), ine)::ih)
+                               (heap_cons 
+*)
   
-Inductive clos_eq : cem.closure → cem.heap → 
-                    Ptr → Ptr → Program → im.Heap → 
-                    Type :=
-  | c_eq : ∀ t e ch p ip ep ih, 
+  
+Open Scope type_scope.
+Fixpoint in_heap_rel (ch : cesm.heap) (ih : im.Heap)
+                     (r : heap_rel ch ih)
+                     (l e ne : nat) (t : db.tm) 
+                     (il ip ep nep : Ptr) : Type := match r with
+  | heap_nil => False
+  | heap_cons l' il' ne' cht iht ip' ep' nep' e' t' _ _ _ _ _ _ rt => 
+    if andb (beq_nat l l') (beq_nat il il') then
+    (ne' = ne) *  (ip' = ip) * (ep' = ep) * (nep' = nep) * (e' = e) * (t' = t)
+    else 
+      if andb (negb (beq_nat l l')) (negb (beq_nat il il'))
+        then in_heap_rel cht iht rt l e ne t il ip ep nep
+        else False
+  end.
+
+Inductive env_eq (ch : cesm.heap) (ih : im.Heap) (r : heap_rel ch ih) (p : Program)
+  : nat → Ptr → Type :=
+  | e0 : env_eq ch ih r p 0 0 
+  | eS : ∀ l e ne t il ip ep nep, 
+    in_heap_rel ch ih r l e ne t il ip ep nep →
+    env_eq ch ih r p l il.
+
+Inductive heap_eq (ch : cesm.heap) (ih : im.Heap) (r : heap_rel ch ih) (p : Program) : Type:=
+  | mkheap_eq : 
+    (∀ l e ne t il ip ep nep, 
+      in_heap_rel ch ih r l e ne t il ip ep nep →
+      (prog_eq ip p t) * 
+      (env_eq ch ih r p e ep) * 
+      (env_eq ch ih r p ne nep)) → 
+    heap_eq ch ih r p.
+
+(*
+Open Scope type_scope.
+Definition zipped := list ((nat * Ptr) * (cell * Ptr * Ptr * Ptr)).
+Fixpoint zipHeaps (ch : cesm.heap) (ih : im.Heap) : zipped := match ch, ih with
+    | (l,c)::ch, (l0,ip)::(l1,ep)::(l2,ine)::ih => 
+        if andb (beq_nat l1 (1+l0)) (beq_nat l2 (2+l0)) then
+        ((l, l0), (c, ip, ep, ine))::zipHeaps ch ih
+        else nil
+    | _, _ => nil
+    end.
+
+Fixpoint lookupZip (key: (nat * Ptr)) (z: zipped)  : 
+  option (cell * Ptr * Ptr * Ptr) := match z,key with
+  | nil, _ => None
+  | ((x,y),v)::xs, (x',y') => if andb (beq_nat x x') (beq_nat y y') then Some v else
+    lookupZip key xs
+  end.
+
+Lemma luz_lu : ∀ ch ih l l' c i e n, 
+  lookupZip (l, l') (zipHeaps ch ih) = Some (c, i, e ,n) →
+  lookup l ch = Some c →
+  lookup l ih = Some i →
+  lookup (1+l) ih = Some e →
+  lookup (1+l) ih = Some n.
+induction ch; intros. inversion H. destruct a. simpl in H. destruct ih.
+inversion H. destruct p. destruct ih. invert H. destruct p0. destruct ih. invert
+H. destruct p1. destruct (PeanoNat.Nat.eqb p0 (S p)) eqn:p0sp.  destruct
+(PeanoNat.Nat.eqb p1 (S (S p))). zipHeaps ch ih) eqn:zh. inversion H. destruct a. destruct p. 
+simpl in H. destruct p0. unfolddestruct 
+*)
+
+Lemma in_heap_rel_lookup : ∀ ch ih r l e ne t il ip ep nep, 
+  in_heap_rel ch ih r l e ne t il ip ep nep →
+  (lookup l ch = Some (cl (close t e) ne)) *
+  (lookup il ih = Some ip) *
+  (lookup (1+il) ih = Some ep) *
+  (lookup (2+il) ih = Some nep).
+intros. induce r. invert X. 
+simpl in X. destruct (eq_nat_dec l0 l). destruct (eq_nat_dec il l'). subst. 
+repeat (rewrite <- beq_nat_refl in X). simpl in X. repeat (destruct X as [X]).
+subst. rewrite lookup_head. rewrite lookup_head. rewrite lookup_head'; auto. 
+rewrite lookup_head. rewrite lookup_head'. rewrite lookup_head'. rewrite
+lookup_head. crush. crush. crush. subst. rewrite <- beq_nat_refl in X. 
+rewrite <- PeanoNat.Nat.eqb_neq in n3. repeat (rewrite n3 in X). simpl in X.
+invert X. destruct (eq_nat_dec il l'). subst. rewrite <- PeanoNat.Nat.eqb_neq in
+n3. rewrite n3 in X. rewrite <- beq_nat_refl in X. simpl in X. invert X. 
+rewrite <- PeanoNat.Nat.eqb_neq in n3.  rewrite <- PeanoNat.Nat.eqb_neq in n4.
+rewrite n3 in X. rewrite n4 in X. simpl in X. apply IHr in X. inversion X.
+invert H. invert H1.  
+apply lookup_domain in H0. apply lookup_domain in H2. apply lookup_domain in H.
+apply lookup_domain in H3. 
+pose (in_notin_neq _ _ _ H0 n0). 
+pose (in_notin_neq _ _ _ H0 n1). 
+pose (in_notin_neq _ _ _ H0 n2). 
+pose (in_notin_neq _ _ _ H2 n0). 
+pose (in_notin_neq _ _ _ H2 n1).
+pose (in_notin_neq _ _ _ H2 n2). 
+pose (in_notin_neq _ _ _ H3 n0). 
+pose (in_notin_neq _ _ _ H3 n1). 
+pose (in_notin_neq _ _ _ H3 n2). 
+pose (in_notin_neq _ _ _ H n). 
+repeat (rewrite lookup_head'; auto). 
+Qed.
+
+(*
+Open Scope type_scope. 
+Lemma heap_rel_lookup : ∀ l l' ne ch ih ip ep ine e t, 
+  heap_rel l e ne t l' ip ep ine ch ih → 
+  (lookup l ch = Some (cl (close t e) ne)) *
+  (lookup l' ih = Some ip) * 
+  (lookup (1+l') ih = Some ep) *
+  (lookup (2+l') ih = Some ine).
+intros. induce X. 
+split. split. split. apply lookup_head. apply lookup_head. rewrite lookup_head';
+auto. apply lookup_head. rewrite lookup_head'; auto. rewrite lookup_head'. apply
+lookup_head. simpl. auto. induction l'; auto. simpl. auto. destruct IHX.
+destruct p. destruct p. split. split. split.  rewrite lookup_head'; auto.
+rewrite lookup_head'; auto. rewrite lookup_head'; auto.  rewrite lookup_head';
+auto. simpl. rewrite lookup_head'; auto. rewrite lookup_head'; auto. rewrite
+lookup_head'; auto. repeat (rewrite lookup_head'; auto). simpl. crush. crush.
+Qed.  
+
+Inductive env_eq' : nat → cesm.heap → Program → Ptr → im.Heap → Type :=
+  | e0 : ∀ h ih p, env_eq' 0 h p 0 ih
+  | en : ∀ l e ne t il ip ie ine h ih p,
+    heap_rel l e ne t il ip ie ine h ih →  
+    prog_eq ip p t →
+    env_eq' e h p ie ih →
+    env_eq' ne h p ine ih →
+    env_eq' l h p il ih.
+*)   
+
+Inductive clos_eq (ch : cem.heap) (ih : im.Heap) (r : heap_rel ch ih) (p : Program):
+                  closure → Ptr → Ptr → Type :=
+  | c_eq : ∀ t e ip ep, 
            prog_eq ip p t → 
-           env_eq e ch p ep ih →
-           clos_eq (cem.close t e) ch ip ep p ih.
+           env_eq ch ih r p e ep →
+           clos_eq ch ih r p (cem.close t e) ip ep. 
 
-Inductive stack_eq : cesm.stack → cesm.heap →
-                     im.Stack → Program → im.Heap → Type := 
-  | stack_nil : ∀ ch p ih, 
-                stack_eq nil ch nil p ih
-  | stack_upd : ∀ e ch p ep ih cs is, 
-                 env_eq e ch p ep ih →
-                 stack_eq cs ch is p ih →
-                 stack_eq (inr e::cs) ch (0::ep::is) p ih
-  | stack_arg : ∀ ch p ip ep ih cs is c, 
-                 clos_eq c ch ip ep p ih →
-                 stack_eq cs ch is p ih → 
-                 stack_eq (inl c::cs) ch (S ip::ep::is) p ih.
+Inductive stack_eq (ch : cem.heap) (ih : im.Heap) (r : heap_rel ch ih) (p : Program) : 
+  cesm.stack → im.Stack → Type := 
+  | stack_nil : stack_eq ch ih r p nil nil
+  | stack_upd : ∀ l e ne t il ip ie ine cs is, 
+                in_heap_rel ch ih r l e ne t il ip ie ine →
+                stack_eq ch ih r p cs is →
+                stack_eq ch ih r p (inr l::cs) (0::il::is)
+  | stack_arg : ∀ ip ep cs is c, 
+                 ip > 0 →
+                 clos_eq ch ih r p c ip ep →
+                 stack_eq ch ih r p cs is → 
+                 stack_eq ch ih r p (inl c::cs) (ip::ep::is).
 
-Inductive state_rel : cesm.state → im.State → Type := 
-  | str : ∀ cs is, 
-  clos_eq (st_cl cs) (st_hp cs) (rff (st_rf is) IP) (rff (st_rf is) EP) (st_p is) (st_h is) →
-  stack_eq (st_st cs) (st_hp cs) (st_s is) (st_p is) (st_h is) →
+Inductive state_rel (cs : cesm.state) (is : im.State) : Type := 
+  | str : ∀ r, 
+  heap_eq (st_hp cs) (st_h is) r (st_p is) →
+  clos_eq (st_hp cs) (st_h is) r (st_p is) (st_cl cs) (rff (st_rf is) IP) (rff (st_rf is) EP) →
+  stack_eq (st_hp cs) (st_h is) r (st_p is) (st_st cs) (st_s is) →
   state_rel cs is.
 
 Lemma skipn_nth_error {A} : ∀ y l (x:A) xs, skipn y l = x::xs → nth_error l y = Some x. 
@@ -63,6 +219,38 @@ induction y; intros. simpl in H. simpl. destruct l. invert H. invert H. auto.
 simpl in H. destruct l. invert H. simpl. apply IHy with (x:=x) (x1:=x1) (xs:=xs). assumption. 
 Qed. 
 
+Lemma firstn_pref {a}: ∀ x y:list a, x = firstn (length x) y → ∃ z, y = x ++ z. 
+induction x; intros. exists y. auto. 
+simpl in H. destruct y. invert H. invert H. rewrite <- H2. apply IHx in H2.
+destruct H2. exists x0. simpl. subst. f_equal. 
+Qed.   
+
+Lemma firstn_app_length {a} : ∀ (x y:list a) p, x ++ y = firstn (length (x ++ y)) p → 
+  x = firstn (length x) p ∧ y = firstn (length y) (skipn (length x) p). 
+intros. apply firstn_pref in H. destruct H. subst. rewrite <- app_assoc.
+generalize dependent y. generalize dependent x0. induction x; intros. simpl.
+split; auto. induction y. simpl. reflexivity. simpl. rewrite <- IHy.
+reflexivity. simpl. split. f_equal. destruct (IHx x0 y). assumption. destruct
+(IHx x0 y). assumption. Qed. 
+
+Lemma skipn_cons {a} : ∀ xs (x:a) n, skipn (S n) (x::xs) = skipn n xs. 
+induction xs; intros. simpl. reflexivity. simpl. reflexivity. 
+Qed.  
+
+Lemma skipn_cons' {a} : ∀ n xs (x:a) ys, skipn n ys = (x::xs) → skipn (S n) ys = xs.
+induction n; intros. simpl. simpl in H. subst. reflexivity. destruct ys. simpl
+in H. invert H. simpl in H. apply IHn in H. rewrite skipn_cons. assumption.  
+Qed.  
+
+Lemma skipn_nil {a} : ∀ n, skipn n (@nil a) = (@nil a). 
+intros. destruct n; auto. Qed. 
+
+Lemma skipnm_add {a} : ∀ m n (xs:list a), skipn n (skipn m xs) = skipn (n + m) xs.
+induction m; intros. simpl. rewrite <- plus_n_O. reflexivity. rewrite
+PeanoNat.Nat.add_comm. simpl. destruct xs. apply skipn_nil. rewrite
+PeanoNat.Nat.add_comm. apply IHm. Qed. 
+
+Open Scope nat_scope. 
 Lemma fresh_closure : ∀ ip ep e f h, (∀ i, lt i 3 → (i+f) ∉ domain h) → 
   replace beq_nat (2+f) e (replace beq_nat (1+f) ep (replace beq_nat f ip 
     ((f,0)::(S f, 0)::(S (S f), 0)::h))) = (f,ip)::(S f, ep)::(S (S f), e)::h.
@@ -87,29 +275,480 @@ unfold replace in *. unfold map in *.
 rewrite H0. rewrite H1. rewrite H2. reflexivity. 
 Qed. 
 
+Lemma lu_update_none : ∀ Φ l l' v, lookup l Φ = None → lookup l (update Φ l' v) = None.
+induction Φ; intros. simpl. unfold lookup. unfold find. reflexivity.
+destruct a. destruct c. destruct (eq_nat_dec l' n). subst. simpl. rewrite
+<- beq_nat_refl. destruct (eq_nat_dec l n). subst. rewrite lookup_head in H.
+invert H. rewrite lookup_head' in H; auto. rewrite lookup_head'; auto. unfold
+update. rewrite <- PeanoNat.Nat.eqb_neq in n0. rewrite n0. destruct (eq_nat_dec
+l n). subst. rewrite lookup_head in H. invert H. rewrite lookup_head'; auto.
+apply IHΦ. rewrite lookup_head' in H; auto. 
+Qed. 
+
+Lemma lu_replace_none {a} : ∀ h l l' (v:a), lookup l h = None → 
+  lookup l (replace beq_nat l' v h) = None.
+induction h; intros. simpl. unfold lookup. unfold find. reflexivity.
+destruct a0. destruct (eq_nat_dec l' n). subst. simpl. rewrite
+<- beq_nat_refl. destruct (eq_nat_dec l n). subst. rewrite lookup_head in H.
+invert H. rewrite lookup_head' in H; auto. rewrite lookup_head'; auto. unfold
+update. rewrite <- PeanoNat.Nat.eqb_neq in n0. unfold replace. simpl. rewrite
+n0. destruct (eq_nat_dec l n). subst. rewrite lookup_head in H. invert H.
+rewrite lookup_head'; auto. unfold replace in IHh. apply IHh. rewrite
+lookup_head' in H; auto.  Qed. 
+
+Lemma update_head : ∀ l c ne h v, update (l ↦ cl c ne::h) l v = 
+                                  l ↦ cl v ne::update h l v. 
+intros. unfold update. rewrite <- beq_nat_refl. reflexivity. 
+Qed. 
+
+Lemma update_head' : ∀ l c ne h v l', 
+  l <> l' →
+  update (l' ↦ cl c ne::h) l v = 
+  l' ↦ cl c ne::update h l v. 
+intros. unfold update. rewrite <- PeanoNat.Nat.eqb_neq in H. rewrite H. reflexivity. 
+Qed. 
+
+Lemma replace_head {a} : ∀ l (y x:a) h, replace beq_nat l x ((l,y)::h) = 
+                                        (l,x)::replace beq_nat l x h.
+intros. unfold replace. simpl. rewrite <- beq_nat_refl. reflexivity. Qed. 
+
+Lemma replace_head' {a} : ∀ l (y x:a) h l',  l <> l' →
+  replace beq_nat l x ((l',y)::h) = 
+  (l',y)::replace beq_nat l x h.
+intros. unfold replace. simpl. rewrite <- PeanoNat.Nat.eqb_neq in H. rewrite H. 
+reflexivity. Qed. 
+
+Lemma update_head_exists : ∀ l l' c ne v h, sigT (λ c', update ((l', cl c ne)::h) l v =
+  (l', cl c' ne)::update h l v).
+intros. simpl. destruct (beq_nat l l'). exists v; auto. exists c; auto. Qed.
+
+Lemma replace_head_exists {a} : ∀ l l' (x:a) h v, sigT (λ y, replace beq_nat l v ((l', x)::h) =
+  (l', y)::replace beq_nat l v h).
+intros. simpl. destruct (beq_nat l l'). exists v; auto. exists x; auto. Qed.
+
+Lemma in_heap_cons : ∀ prop ch ih r l' e' ne' t' il' ip' ep' nep', 
+  (∀ l e ne t il ip ep nep, 
+    in_heap_rel ch ih r l e ne t il ip ep nep → 
+    prop l e ne t il ip ep nep) → 
+  ∀ pl pil pil1 pil2 plg pilg,
+  prop l' e' ne' t' il' ip' ep' nep' →
+  (∀ l e ne t il ip ep nep, 
+    in_heap_rel ((l', cl (close t' e') ne')::ch) 
+                ((il', ip')::(S il',ep')::(S (S il'),nep')::ih) 
+                (heap_cons _ _ _ _ _ _ _ _ _ _ pl pil pil1 pil2 plg pilg r) 
+                l e ne t il ip ep nep →
+    prop l e ne t il ip ep nep).
+intros. simpl in X1. destruct (beq_nat l l') eqn:ll'. destruct (beq_nat il il')
+eqn:ilil'. simpl in X1. repeat (destruct X1 as [X1]). apply beq_nat_true in ll'.
+apply beq_nat_true in ilil'. subst. assumption. simpl in X1. invert X1. destruct
+(beq_nat il il') eqn:ilil'. simpl in X1. invert X1. simpl in X1. apply X in X1.
+assumption. Qed.
+
+Lemma in_heap_head : ∀ l l' ne ch ih ip ep ine e t f0 f1 f2 f3 f4 f5 r, 
+  in_heap_rel ((l, cl (close t e) ne)::ch) 
+              ((l', ip)::(S l', ep)::(S (S l'), ine)::ih)    
+    (heap_cons l l' ne ch ih ip ep ine e t f0 f1 f2 f3 f4 f5 r)
+    l e ne t l' ip ep ine.
+intros. simpl. rewrite <- beq_nat_refl. rewrite <- beq_nat_refl. simpl. crush. 
+Qed. 
+    
+Lemma in_heap_rel_upd_head : 
+  ∀ l l' il il' t t' e e' ne ne' ip ep nep ip' ep' nep' ch ih r pl pil psil
+  pssil gl gil, 
+  in_heap_rel ((l, cl (close t e) ne)::ch) 
+              ((il, ip)::(S il, ep)::(S (S il), nep)::ih)
+              (heap_cons l il ne ch ih ip ep nep e t pl pil psil pssil gl gil r)
+              l' e' ne' t' il' ip' ep' nep' → 
+  (l = l') * (ne = ne') * (il = il') * (nep = nep') * (t = t') * (e = e') * (ip = ip') * (ep = ep') + 
+  (l ≠ l') * (il ≠ il') * (S il ≠ il') * (S (S il) ≠ il') * in_heap_rel ch ih r l' e' ne' t' il' ip' ep' nep'. 
+intros. simpl in X.  destruct (eq_nat_dec l l'); destruct (eq_nat_dec il il').
+subst. rewrite <- beq_nat_refl in X. rewrite <- beq_nat_refl in X. simpl in X.
+crush. rewrite <- PeanoNat.Nat.eqb_neq in n. rewrite beq_nat_comm in n. rewrite
+n in X.  simpl in X. subst. rewrite <- beq_nat_refl in X.  simpl in X. invert X.
+subst. rewrite <- PeanoNat.Nat.eqb_neq in n. rewrite beq_nat_comm in n. rewrite
+n in X. simpl in X. rewrite <- beq_nat_refl in X. simpl in X. invert X. apply
+inr. apply prod_assoc'. apply prod_assoc'. split. crush. rewrite <-
+PeanoNat.Nat.eqb_neq in n. rewrite <- PeanoNat.Nat.eqb_neq in n0.  rewrite
+beq_nat_comm in n. rewrite beq_nat_comm in n0. rewrite n in X.  rewrite n0 in X.
+simpl in X. apply prod_assoc.  split. apply in_heap_rel_lookup in X. destruct X. destruct p.
+destruct p. apply lookup_domain in e4. split. unfold not. intros. subst. apply
+psil in e4. invert e4. unfold not. intros. subst. apply pssil in e4. invert e4.
+assumption. Qed.  
+
+Lemma in_heap_rel_upd_head' :
+  ∀ l l' il il' t t' e e' ne ne' ip ep nep ip' ep' nep' ch ih r pl pil psil
+  pssil gl gil, 
+  (l = l') * (ne = ne') * (il = il') * (nep = nep') * (t = t') * (e = e') * (ip = ip') * (ep = ep') + 
+  (l ≠ l') * (il ≠ il') * in_heap_rel ch ih r l' e' ne' t' il' ip' ep' nep' →
+  in_heap_rel ((l, cl (close t e) ne)::ch) 
+              ((il, ip)::(S il, ep)::(S (S il), nep)::ih)
+              (heap_cons l il ne ch ih ip ep nep e t pl pil psil pssil gl gil r)
+              l' e' ne' t' il' ip' ep' nep'. 
+intros. destruct X. crush. rewrite <- beq_nat_refl. rewrite <- beq_nat_refl.
+simpl. crush. destruct p. simpl. destruct p. rewrite <- PeanoNat.Nat.eqb_neq in
+n. rewrite <- PeanoNat.Nat.eqb_neq in n0. rewrite beq_nat_comm. rewrite n.
+rewrite beq_nat_comm. rewrite n0. simpl. assumption. Qed.
+
+Lemma forall_heap_rel_tail : ∀ l il t e ne ip ep nep ch ih
+  r pl pil psil pssil gl gil prop, 
+  (∀ l' e' ne' t' il' ip' ep' nep', in_heap_rel 
+    ((l, cl (close t e) ne)::ch) 
+    ((il, ip)::(S il, ep)::(S (S il), nep)::ih) 
+    (heap_cons l il ne ch ih ip ep nep e t pl pil psil pssil gl gil r) 
+    l' e' ne' t' il' ip' ep' nep' →
+    prop t' e' ip' ep') → 
+  (∀ l' e' ne' t' il' ip' ep' nep', in_heap_rel 
+    ch 
+    ih 
+    r 
+    l' e' ne' t' il' ip' ep' nep' →
+    prop t' e' ip' ep'). 
+intros. apply X with (l':=l') (ne':=ne') (il':=il') (nep':=nep'). apply
+in_heap_rel_upd_head'. apply inr. split; auto. apply in_heap_rel_lookup
+in X0. destruct X0. destruct p. destruct p. apply lookup_domain in e3. apply
+lookup_domain in e4. split; (unfold not; intros; subst). 
+apply pl in e3. assumption. apply pil in e4. assumption. 
+Qed. 
+
+Lemma contractable_heap_rel : ∀ ch ih (r1 r2: heap_rel ch ih), r1 = r2.  
+intros. induce r1. dependent destruction r2. reflexivity. dependent destruction
+r2. 
+rewrite (proof_irrelevance _ n n3). 
+rewrite (proof_irrelevance _ n0 n4). 
+rewrite (proof_irrelevance _ n1 n5). 
+rewrite (proof_irrelevance _ n2 n6). 
+rewrite (proof_irrelevance _ g g1). 
+rewrite (proof_irrelevance _ g0 g2). 
+rewrite (IHr1 r2). reflexivity. 
+Qed. 
+
+Lemma in_heap_rel_upd : ∀ ch ih r l e ne t il ip ep nep ep' ip' v e' 
+  (prop : tm → nat → Ptr → Ptr → Type),
+  (∀ l e ne t il ip ep nep, in_heap_rel ch ih r l e ne t il ip ep nep → 
+                            prop t e ip ep) →
+  in_heap_rel ch ih r l e ne t il ip ep nep →
+  prop v e' ip' ep' →
+  sigT (λ r', (∀ l' e ne t il' ip ep nep, 
+      (in_heap_rel (update ch l (close v e')) 
+                  (replace beq_nat (S il) ep' (replace beq_nat il ip' ih)) 
+                  r' l' e ne t il' ip ep nep) → prop t e ip ep)).
+intros. induce r. invert X0. assert (X0' := X0). apply in_heap_rel_upd_head in
+X0'. destruct X0'. 
+- repeat (destruct p). subst. rewrite update_head. rewrite replace_head. rewrite
+  replace_head'; auto.  rewrite replace_head'; auto. rewrite replace_head.
+  rewrite replace_head'.  rewrite replace_head'.  rewrite replace_not_in.
+  rewrite replace_not_in. rewrite update_nodomain; auto. 
+  exists (heap_cons l0 il ne0 ch ih ip' ep' nep e' v n n0 n1 n2 g g0 r).
+  intros. apply in_heap_rel_upd_head in X2. destruct X2. repeat
+  destruct p. subst. assumption. apply (X l' _ ne _ il' _ _ nep0). apply
+  in_heap_rel_upd_head'. apply inr. crush. auto. rewrite replace_not_in.
+  assumption. assumption. auto. crush.   
+- assert (n' := n). 
+  assert (n0' := n0). 
+  assert (n1' := n1).
+  assert (n2' := n2). 
+  rewrite <- domain_update with (l:=l0) (v:=close v e') in n'. 
+  rewrite replace_domain with (l1:=il) (eq0:=beq_nat) (v0:=ip') in n0'. 
+  rewrite replace_domain with (l1:=S il) (eq0:=beq_nat) (v0:=ep') in n0'.
+  rewrite replace_domain with (l1:=il) (eq0:=beq_nat) (v0:=ip') in n1'. 
+  rewrite replace_domain with (l1:=S il) (eq0:=beq_nat) (v0:=ep') in n1'.
+  rewrite replace_domain with (l1:=il) (eq0:=beq_nat) (v0:=ip') in n2'. 
+  rewrite replace_domain with (l1:=S il) (eq0:=beq_nat) (v0:=ep') in n2'.
+  specialize (IHr l0 e1 ne0 t0 il ip0 ep0 nep ep' ip' v e' prop).
+  destruct p. repeat (destruct p).  
+  rewrite update_head'. Focus 2. crush. 
+  repeat (rewrite replace_head'; auto). Focus 2. apply in_heap_rel_lookup in i.
+  destruct i. repeat (destruct p). simpl in e3. apply lookup_domain in e3. apply
+  (in_notin_neq (S il) l' (domain ih)); auto.  
+  assert (ihr := forall_heap_rel_tail _ _ _ _ _ _ _ _ _ _ _ _ _ _ _ _ _ _ X). 
+  specialize (IHr ihr i X1). destruct IHr. 
+  exists (heap_cons l l' ne 
+         (update ch l0 (close v e')) 
+         (replace beq_nat (S il) ep' (replace beq_nat il ip' ih))
+         ip ep ine e t n' n0' n1' n2' g g0 x).
+  intros. 
+  apply in_heap_rel_upd_head in X2. destruct X2.   
+  repeat (destruct p0). subst. assert (ihh := in_heap_head). apply X in ihh.
+  assumption. repeat (destruct p0). (*rewrite (contractable_heap_rel _ _ r' x) in
+  i0.*) apply p in i0. assumption. 
+  Qed. 
+
+Lemma in_heap_rel_upd : ∀ ch ih r l e ne t il ip ep nep ep' ip' v p e', 
+  in_heap_rel ch ih r l e ne t il ip ep nep →
+  heap_eq ch ih r p → 
+  prog_eq ip' p v →
+  env_eq ch ih r p e' ep' → 
+  sigT (λ r', heap_eq (update ch l (close v e'))
+          (replace beq_nat (S il) ep' (replace beq_nat il ip' ih))
+          r'
+          p).
+intros. induce r. 
+- simpl. exists heap_nil. constructor. simpl. intros. invert H0.      
+- invert X0. apply in_heap_rel_upd_head in X. destruct X. 
+  + repeat (destruct p0).     exists (heap_cons l0 il ne0 ch ih ip' ep' nep e' v n n0 n1 n2 g g0 r).
+    specialize (X2 _ _ _ _ _ _ _ _ (in_heap_head _ _ _ _ _ _ _ _ _ _ _ _ _ _ _ _
+    _)).  constructor. intros. apply in_heap_rel_upd_head in X. destruct X.
+    crush. eapply (eS _ _ _ p e1 e ne t il0 ip ep nep0 _) .  crush. specialize
+    (X2 l e1 ne t0 il0 ip0 ep0 nep0).
+    rewrite <- beq_nat_refl in X2. rewrite <- beq_nat_refl in X2. simpl in X2.
+    crush. const assumption. split. split.  h
+    assumption. 
+    rewrite
+  replace_head. simpl. rewrite <- beq_nat_refl. rewrite <-
+  beq_nat_refl. destruct il. crush p0. pply X2 in X. destruct X. destruct p0. apply in_heap_rel_upd_head
+  in X2. simpl. simpl in 
+  destruct (beq_nat l0 l) eqn:l0l.             
+  destruct (beq_nat il l') eqn:ill'. simpl in X. apply beq_nat_true in l0l. apply
+beq_nat_true in ill'. subst. repeat (destruct X as [X]). subst. 
+rewrite update_head. rewrite replace_head. rewrite
+replace_head'; auto. rewrite replace_head'; auto. rewrite replace_head. rewrite
+replace_head'; auto. rewrite replace_head'; auto. 
+rewrite update_nodomain; auto. repeat (rewrite replace_not_in); auto. 
+eapply (existT _ (heap_cons l l' ne ch ih ip' ep' ine e' v n n0 n1 n2 r)).
+constructor. apply in_heap_cons.    
+constructor. intros. simpl in X0. destruct (beq_nat l0 l) eqn:l0l. destruct
+(beq_nat il l') eqn:ill'. simpl in X0. crush.   
+subst. pose r. eapply heap_cons in h; auto. exists
+h. constructor. intros. destruct X0. simpl in p0. inversion h. subst. unfold
+in_heap_rel in X. simpl in X. destruct X0. assumption.  assert (ch = update ch l
+(close v e')). symmetry. apply update_nodomain.  assumption. rewrite H0 in h.
+assert (replace beq_nat (S l') ep' (replace 
+destruct X0. eapply heap_cons;
+auto. rewrite domain_update. assumption. rewrite <- replace_domain. rewrite
+<- replace_domain. assumption. rewrite <- replace_domain. rewrite <-
+replace_domain. assumption. repeat (rewrite <- replace_domain). assumption. 
+rewrite update_nodomain; auto. repeat (rewrite replace_not_in; auto). crush.
+simpl in X. invert X. destruct (PeanoNat.Nat.eqb il l') eqn:ill'. simpl in X. invert X. 
+simpl in X. apply beq_nat_false in l0l. apply beq_nat_false in ill'. rewrite
+update_head'; auto. specialize (IHr _ _ _ _ _ _ _ _ ep' ip' v X). 
+apply in_heap_rel_lookup in X. destruct X. destruct p. destruct p. apply
+lookup_domain in e4. apply lookup_domain in e5. apply lookup_domain in e3. apply
+lookup_domain in e2.  
+pose (in_notin_neq _ _ _ e4 n). 
+pose (in_notin_neq _ _ _ e5 n0). 
+pose (in_notin_neq _ _ _ e5 n1). 
+pose (in_notin_neq _ _ _ e5 n2). 
+pose (in_notin_neq _ _ _ e2 n0). 
+pose (in_notin_neq _ _ _ e2 n1).
+pose (in_notin_neq _ _ _ e2 n2). 
+pose (in_notin_neq _ _ _ e3 n0). 
+pose (in_notin_neq _ _ _ e3 n1). 
+pose (in_notin_neq _ _ _ e3 n2). 
+repeat (rewrite replace_head'; auto). apply heap_cons;
+auto.  rewrite domain_update. assumption. repeat (rewrite <- replace_domain).
+assumption. repeat (rewrite <- replace_domain). assumption. repeat (rewrite <-
+replace_domain). assumption.
+Qed.
+
+Lemma heap_eq_update' : ∀ ch ih r l e ne t il ip ep nep ep' ip' v p e'
+  (ihr : in_heap_rel ch ih r l e ne t il ip ep nep),
+  heap_eq ch ih r p → 
+  prog_eq ip' p v →
+  env_eq ch ih r p e' ep' →
+  heap_eq (update ch l (close v e'))
+          (replace beq_nat (S il) ep' (replace beq_nat il ip' ih))
+          (in_heap_rel_upd ch ih r l e ne t il ip ep nep ep' ip' (close v e') ihr)
+          p.
+intros. induce r. invert ihr. invert X. simpl. unfold in_heap_rel_up. simpl in X1.split. split. split.  simpl
+in ihr. simpl. 
+
+
+Lemma heap_rel_update' : ∀ l e ne t il ip ie ine Φ ih l' il' ep' ip' v,
+  l <> l' → il <> il' → S il <> il' → S (S il) <> il' → il <> S il' → il <> S (S
+  il') →
+  heap_rel l e ne t il ip ie ine Φ ih →
+  heap_rel l e ne t il ip ie ine (update Φ l' v) (replace beq_nat (S il') ep'
+  (replace beq_nat il' ip' ih)).
+intros. induce X. rewrite update_head'; auto. repeat (rewrite replace_head');
+auto. constructor.  
++ subst. destruct c'. edestruct update_head_exists. rewrite e1. 
+edestruct (@replace_head_exists nat). rewrite e2. clear e2. 
+edestruct (@replace_head_exists nat). rewrite e2. clear e2. 
+edestruct (@replace_head_exists nat). rewrite e2. clear e2. 
+edestruct (@replace_head_exists nat). rewrite e2. clear e2. 
+edestruct (@replace_head_exists nat). rewrite e2. clear e2. 
+edestruct (@replace_head_exists nat). rewrite e2. clear e2. 
+constructor; auto. 
+Qed.
+  
+Open Scope type_scope. 
+Lemma heap_rel_update : ∀ l e ne t il ip ie ine Φ ih
+                          l' e' ne' t' il' ip' ie' ine'
+                          t'' e'' ie'' ip'',
+  heap_rel l e ne t il ip ie ine Φ ih →  
+  heap_rel l' e' ne' t' il' ip' ie' ine' Φ ih →
+  ∃ ne, heap_rel l' e'' ne' t'' il' ip'' ie'' ine'
+        (update Φ l (close t'' e'')) 
+        (replace beq_nat (S il) ie''
+        (replace beq_nat il ip'' ih))) 
+                      +
+  ((l <> l') * (il <> il') * heap_rel l' e' ne' t' il' ip' ie' ine'
+        (update Φ l (close t'' e''))
+        (replace beq_nat (S il) ie''
+        (replace beq_nat il ip'' ih))).
+intros. induce X. induce X0. invert H1. invert H0. apply inl. split; auto.
+rewrite update_head. rewrite replace_head. rewrite replace_head'; auto. rewrite
+replace_head'; auto. rewrite replace_head. rewrite replace_head'. rewrite
+replace_head'; auto. constructor. crush. invert H1. invert H0. apply inr. split;
+auto. rewrite update_head. rewrite replace_head. rewrite replace_head'; auto.
+rewrite replace_head'; auto. rewrite replace_head. repeat (rewrite
+replace_head'; auto).  constructor; auto.  apply heap_rel_update'. auto. auto.
+auto. auto. auto. auto.  auto. crush. auto. crush. 
+simpl in X0. destruct c'. apply heap_rel_update' with (l':=l) (v:=close t''
+e'') (il':=l') (ep':=ie'') (ip':=ip'') in X0. 
+rewrite update_head'; auto. repeat (rewrite replace_head'; auto). 
+rewrite update_head' in X0; auto.  repeat (rewrite replace_head' in X0;
+auto).    
+edestruct IHX . eapply heap_rel_update' in X. eapply X. 
+edestruct update_head_exists. rewrite e1 in *. 
+edestruct (@replace_head_exists nat). rewrite e2 in *. clear e2. 
+edestruct (@replace_head_exists nat). rewrite e2 in *. clear e2. 
+edestruct (@replace_head_exists nat). rewrite e2 in *. clear e2. 
+edestruct (@replace_head_exists nat). rewrite e2 in *. clear e2. 
+edestruct (@replace_head_exists nat). rewrite e2 in *. clear e2. 
+edestruct (@replace_head_exists nat). rewrite e2 in *. clear e2. 
+edestruct IHX. invert X0. invert e1.  
+*)
+Lemma env_eq_update' : ∀ Φ p ih l il e ep ip c ie ine' ie' ip' t ne e', 
+  clos_eq c Φ ip ep p ih →
+  heap_rel l e' ne t il ip' ie' ine' Φ ih →  
+  env_eq' e Φ p ie ih →
+  env_eq' e (update Φ l c) p ie
+    (replace beq_nat (S il) ep (replace beq_nat il ip ih)).
+intros. invert X. induce X1. constructor. eapply heap_rel_update' in h0.
+econstructor. apply h0. assumption. eapply IHX1_1. apply X0. assumption.
+assumption. eapply IHX1_2. apply X0. assumption. assumption. rewrite
+update_head. rewrite replace_head. rewrite replace_head'; auto. rewrite
+replace_head'; auto. rewrite replace_head. rewrite
+replace_head'; auto. rewrite replace_head'; auto. induce X1. constructor. induce
+h0. invert H1. invert H2. eapply en. constructor; auto. assumption. assumption.  
+eapply en. constructor. induce h0. invert H1. invert H2.  constructor; auto. eapply IHh0.
+apply p0. apply X1_1. induce X1. constructor. econstructor. 
+crush. constructor;
+auto. invert X1. 
+crush.  
+econstructor. apply heap_tail. constructor. constructor. induce X1. constructor. induce h0; intros. 
+constructor. 
+ subst.  unfold update. rewrite <- beq_nat_refl.
+apply heap_head. constructor.
+induce X1; intros. apply e0. apply lu_update_none; auto.  simpl.
+apply lu_replace_none; auto. apply lu_replace_none. auto. eapply en.   
+
+
+simpl in *. 
+induce h0. 
+eapply en. 
+induce h0. 
+apply luhdestruct (eq_nat_dec n l).
+- subst. econstructor. eapply lookup_update. apply e0.      
+Admitted.
+*)
+
+Lemma env_eq_fresh' : ∀ e Φ p ep ih f f' ip0 ep0 ne0 t e' ne',
+  env_eq' e Φ p ep ih → 
+  f > 0 →
+  f ∉ domain Φ →
+  f' ∉ domain ih →
+  (1+f') ∉ domain ih →
+  (2+f') ∉ domain ih →
+  env_eq' e ((f, cl (close t e') ne')::Φ) p ep ((f',ip0)::(1+f',ep0)::(2+f',ne0)::ih).
+intros. induce X. apply e0. eapply en. 
+destruct (heap_rel_lookup _ _ _ _ _ _ _ _ _ _ h0). 
+destruct p1. destruct p1. 
+apply lookup_domain in e3.
+apply lookup_domain in e4. 
+apply lookup_domain in e2. 
+apply lookup_domain in e1. 
+constructor; try (apply neq_sym). 
+eapply in_notin_neq. apply e3. apply H0.  
+eapply in_notin_neq. apply e4. apply H1. 
+eapply in_notin_neq. apply e4. apply H2. 
+eapply in_notin_neq. apply e4. apply H3. 
+eapply in_notin_neq. apply e2. apply H1. 
+eapply in_notin_neq. apply e1. apply H1. 
+apply h0. assumption. 
+apply IHX1; auto. 
+apply IHX2; auto. 
+Qed.
+
+Lemma env_eq_fresh : ∀ e Φ p ep c ih f f' ip0 ep0 ne0,
+  env_eq e Φ p ep ih →
+  f ∉ domain Φ →
+  f' ∉ domain ih →
+  (1+f') ∉ domain ih →
+  (2+f') ∉ domain ih →
+  env_eq f ((f, c)::Φ) p f' ((f',ip0)::(1+f',ep0)::(2+f',ne0)::ih) →
+  env_eq e ((f, c)::Φ) p ep ((f',ip0)::(1+f',ep0)::(2+f',ne0)::ih).
+intros. induce X. simpl. destruct c0. eapply ee. invert X0. intros. destruct (eq_nat_dec n
+f). subst. rewrite lookup_head in H3. invert H3. subst. 
+rewrite lookup_head' in H3; auto.
+repeat (rewrite lookup_head'; auto). apply p0. apply H3. apply lookup_domain in e1. eapply in_notin_neq. apply e1.  assumption.
+rewrite lookup_head'. rewrite lookup_head'. rewrite lookup_head'. apply e2.
+eapply in_notin_neq. apply lookup_domain in e1. apply e1. assumption. 
+eapply in_notin_neq. apply lookup_domain in e1. apply e1. assumption.  
+eapply in_notin_neq. apply lookup_domain in e1. apply e1. assumption.  
+rewrite lookup_head'. rewrite lookup_head'. rewrite lookup_head'. apply e2. 
+eapply in_notin_neq. apply lookup_domain in e2. apply e2. auto. 
+eapply in_notin_neq. apply lookup_domain in e2. apply e2. auto. 
+eapply in_notin_neq. apply lookup_domain in e2. apply e2. auto. 
+rewrite lookup_head'. rewrite lookup_head'. rewrite lookup_head'. apply e3. 
+eapply in_notin_neq. apply lookup_domain in e3. apply e3. auto. 
+eapply in_notin_neq. apply lookup_domain in e3. apply e3. auto. 
+eapply in_notin_neq. apply lookup_domain in e3. apply e3. auto. 
+assumption. apply IHX1; auto. 
+apply IHX2; auto. 
+Qed.
+
 Lemma cesm_im : ∀ v s s', 
   state_rel s s' → 
   cesm.step s v → 
   sigT (λ v', prod (refl_trans_clos im.step s' v') (state_rel v v')).
 intros v s s' r h. induce h. 
-- invert r. invert X. simpl in *. invert X0. destruct s' as [rf p is' h]. simpl
-  in *. subst. exists (st (upd R1 ep rf) p is (replace beq_nat (1 + ep)
-  (im.ep rf) (replace beq_nat ep (ip rf) h))). split.  
-  + apply t_step with (y:=st (upd IP (1 + ip rf) (upd R1 0 rf)) p (ep::is)
-    h). invert H6.  destruct (skipn (ip rf) p) eqn:snip. invert H0. apply enter
-    with (k:=ip rf) (bb:=b0).  constructor. apply skipn_nth_error in snip.
-    assumption. invert H0.  eapply step_pop. constructor.  eapply step_jump0.
-    destruct rf. simpl.  constructor.  constructor.  simpl.  apply t_step with
-    (y:=st (upd R1 ep rf) p is (replace beq_nat (1 + ep) (im.ep rf) (replace
-    beq_nat ep (ip rf) h))).  invert H6.  destruct (skipn (ip rf) p)
-    eqn:skip. inversion H0.  destruct l0 eqn:l0e.  invert H0.  subst. apply
-    skipn_nth_error_1 in skip.  apply enter with (k:=1 + ip rf) (bb:=b1).
-    destruct rf. constructor.  assumption.  inversion H0.  subst.  eapply
-    step_pop.  constructor. eapply step_mov.  constructor. eapply write_mem.
-    eapply step_mov.  constructor.  eapply write_mem. eapply step_jump.
-    constructor.  simpl. destruct rf. simpl in *. eapply write_reg. apply
-    t_refl. 
-  + admit. 
+- invert r. invert X. simpl in *. invert X0. destruct s'. simpl in *. subst.  
+  exists (st (upd R1 ep st_rf) st_p is 
+    (replace beq_nat (1 + ep) (im.ep st_rf) (replace beq_nat ep (ip st_rf) st_h))). 
+  split.  
+  + destruct st_rf; simpl in *. 
+    invert H6.  destruct (skipn ip st_p) eqn:snip. invert H0. 
+    invert H0.  destruct l0. invert H2. invert H2. 
+    eapply t_step. 
+    eapply enter.
+    constructor. 
+    apply skipn_nth_error in snip.
+    simpl. eapply snip. 
+    econstructor. 
+    econstructor. 
+    econstructor. 
+    econstructor. 
+    eapply write_reg. 
+    econstructor. 
+    econstructor. 
+    econstructor. 
+    apply skipn_nth_error_1 in snip.
+    apply snip. 
+    econstructor. 
+    econstructor. 
+    econstructor. 
+    econstructor. 
+    econstructor.
+    econstructor.
+    econstructor.
+    econstructor.
+    econstructor.
+    econstructor.
+    econstructor.
+    simpl.
+    apply t_refl. 
+  + destruct st_rf; simpl in *. induce X1. 
+      destruct (eq_nat_dec n l). 
+    * subst. constructor; simpl. constructor. assumption. econstructor. 
+      eapply lookup_update. apply e0. 
+      destruct (eq_nat_dec p (S ep)). 
+      ** subst.  eapply lookup_replace. apply lookup_replace'. apply e1. auto.
+      ** apply lookup_replace'. 
+         destruct (eq_nat_dec p ep). subst. eapply lookup_replace.  apply
+         (lookup  destruct induce X1. 
+  assumption.*)
 - generalize dependent e0. generalize dependent r. generalize dependent e.
   generalize dependent l. generalize dependent e'. generalize dependent s'.
   generalize dependent c. induction v; intros. 
@@ -120,50 +759,69 @@ intros v s s' r h. induce h.
   e'0 ip r2) st_p (0::ep::st_s) st_h). split. 
     + eapply t_step. eapply enter.
       constructor. apply skip. eapply step_push. constructor. eapply step_push.
-      constructor. eapply step_mov. constructor. simpl. apply H0.  constructor.
+      constructor. eapply step_mov. simpl. eapply read_mem. simpl. apply H0.  constructor.
       eapply step_mov. constructor. simpl. apply H1. constructor.  eapply
       step_jump. constructor. constructor. simpl. eapply t_refl.  
-    + admit. 
+    + constructor; simpl. constructor. assumption. assumption. constructor;
+      auto.   
   * simpl in e0. destruct (lookup e Φ) eqn:lue. destruct c0. eapply (IHv _ _ _ _
     _ _ e0). invert e0.  
 - destruct s'. invert r. simpl in *. invert X. invert X0. destruct st_rf. simpl
-  in *. destruct (new 3 st_h) as [f' ff']. exists (st (mkrf (3+ip0) f (S ip) f')
+  in *. destruct (new 3 st_h) as [f' ff']. exists (st (mkrf (3+ip0) f' ip f')
   st_p is ((f',ip)::(1+f',ep)::(2+f',ep0)::st_h)). split. 
   + eapply t_step. eapply enter; simpl. constructor. simpl. invert H6. destruct
   (skipn ip0 st_p) eqn:skip. invert H0. invert H0. apply skipn_nth_error in
   skip. apply skip. eapply step_pop. constructor. eapply step_jumpS.
-  simpl. eapply (read_reg R1 (st (mkrf ip0 ep0 (S ip) r2) st_p (ep::is) st_h)). 
+  simpl. apply H5. simpl. eapply (read_reg R1 (st (mkrf ip0 ep0 ip r2) st_p (ep::is) st_h)). 
   constructor. constructor. simpl. eapply t_step. eapply enter. constructor. 
   simpl. invert H6. destruct (skipn ip0 st_p) eqn:skip. invert H0. destruct l.
   invert H0. destruct l. invert H0. invert H0. apply skipn_nth_error_2 in skip.
-  apply skip. eapply step_new. apply ff'. repeat (econstructor). eapply step_mov.
-  constructor. constructor. repeat (econstructor). unfold rff. unfold im.r2.
-  unfold upd. unfold im.ep. unfold st_rf. unfold im.r1. rewrite plus_O_n. unfold
-  zeroes. unfold app. rewrite fresh_closure. apply t_refl.  rewrite simpl.  rewrite
-  PeanoNat.Nat.eqb_refl. assert (PeanoNat.Nat.eqb f' (S (S f')) = false). clear ff'. 
-  induction f'; auto. rewrite H. simpl. apply IHf'. assumption. rewrite PeanoNat.Nat.add_comm. simpl.   
-  apply r. . 
-  so
-
-
-
-specialize (IHv _ _
-  * _ _ _ _ lue). invert r. invert X.
-  * jump0.  with
-  (y:=(st (mkrf ip e'0 ip r2) st_p (0::ep::st_s) st_h)). eapply apply 
-  destruct rf. simpl in *. constructor; simpl. constructor. assumption. clear
-  H6. clear X2. induce X1. constructor; simpl. constructor.
-    assumption. destruct (eq_nat_dec n l). subst. eapply ee. apply lookup_update with
-    (c:=close t e). apply e0. apply lookup_update'. apply e0. in e0. . eapply
-    IHX1_2. constructor; simpl. constructor.
-    eapply IHX1_2. assumption.  eapply ee. invert X1.  
-- 
-  constructor.  destruct invert
-  H6. invert H0.  apply enter with (k:=.  apply match r with r
+  apply skip. eapply step_new. apply ff'. econstructor. repeat (econstructor).
+  unfold rff. unfold upd. unfold im.r2. unfold st_rf. unfold im.ep. unfold
+  im.r1. unfold zeroes. unfold app. rewrite (fresh_closure ip ep ep0 f'). apply
+  t_refl. apply ff'.
+  + constructor; simpl. constructor. unfold prog_eq. invert H6. destruct (skipn
+    ip0 st_p) eqn:sn. invert H0. invert H0. destruct l. invert H2. invert H2.
+    destruct l. invert H1. invert H1. rewrite H2 at 1. f_equal. symmetry. eapply
+    skipn_3_skipn. apply sn. destruct c. econstructor. rewrite lookup_head.
+    reflexivity. apply lookup_head. simpl. rewrite lookup_head'; auto. apply
+    lookup_head. rewrite lookup_head'; auto. rewrite lookup_head'; auto. apply
+    lookup_head. simpl. crush. crush. invert X. assumption. apply env_eq_fresh;
+    auto. invert X. assumption. apply (ff' 0). auto. apply env_eq_fresh; auto. 
+    apply (ff' 0). auto. induction X2. constructor. constructor. apply IHX2;
+    auto. constructor. assumption. destruct c1. constructor. assumption.
+    apply env_eq_fresh; auto. apply (ff' 0). auto. apply IHX2; auto. 
+- invert r. invert X. destruct s'. simpl in *. destruct st_rf. simpl in *.
+  invert H6. destruct (skipn ip st_p) eqn:skip. invert H0. remember (skipn_nth_error
+  _ _ _ _ skip). clear Heqe0. exists (st (mkrf (S ip) ep r1 r2) st_p (S ip + length (assemble
+  m (S ip))::ep::st_s) st_h). invert H0. split. 
+  + eapply t_step.  
+    econstructor. 
+    constructor.
+    simpl. apply e0.  
+    econstructor. 
+    econstructor. 
+    econstructor. 
+    econstructor. 
+    econstructor. 
+    econstructor.
+    econstructor. 
+    apply t_refl.  
+  + constructor; simpl. constructor. unfold prog_eq. apply firstn_app_length in
+    H2. destruct H2. rewrite H at 1. simpl. induction st_p. destruct ip. invert
+    skip. invert skip. destruct ip. invert skip. simpl. reflexivity. simpl in
+    skip. apply skipn_cons' in skip.  rewrite skip. reflexivity. assumption.
+    constructor. apply Gt.gt_Sn_O. constructor; auto. unfold prog_eq. apply
+    firstn_app_length in H2. destruct H2. apply skipn_cons' in skip. subst.
+    rewrite H0 at 1. f_equal. rewrite skipnm_add. rewrite PeanoNat.Nat.add_comm.
+    simpl. reflexivity. assumption. 
 Admitted.
 
+
+(*
 Lemma cesm_im_assemble : ∀ t v v', 
   refl_trans_clos cesm.step (cesm.I t) v → 
   refl_trans_clos im.step (im.I (assemble t 1)) v'.
-Admitted.
+*)
+
 
