im.v
@@ -7,32 +7,37 @@ Require Import util.
 
 Definition Heap := Map Ptr Word.
 Definition Stack := list Word.
-Definition RegisterFile := Reg → Ptr.
 
 (*
-Inductive RegisterFile := rf {
-  ip : Ptr;
-  ep : Ptr;
-  r1 : Ptr; 
-  r2 : Ptr;
-  r3 : Ptr
-}. 
-
-Definition rff (r: Reg) : RegisterFile → Ptr := match r with
-  | IP => ip 
-  | EP => ep
-  | R1 => r1
-  | R2 => r2
-  | R3 => r3
-  end.
-*)
-
+Definition RegisterFile := Reg → Ptr.
 Definition upd (r: Reg) (p: Ptr) (rf: RegisterFile) : RegisterFile := match r with
   | IP => λ r, match r with | IP => p | _ => rf r end
   | EP => λ r, match r with | EP => p | _ => rf r end
   | R1 => λ r, match r with | R1 => p | _ => rf r end
   | R2 => λ r, match r with | R2 => p | _ => rf r end
   | R3 => λ r, match r with | R3 => p | _ => rf r end
+  end.
+*)
+
+Inductive RegisterFile := mkrf {
+  ip : Ptr;
+  ep : Ptr;
+  r1 : Ptr; 
+  r2 : Ptr
+}. 
+
+Definition upd (r: Reg) (p: Ptr) (rf: RegisterFile) : RegisterFile := match r,rf with
+  | IP, mkrf ip ep r1 r2 => mkrf p ep r1 r2
+  | EP, mkrf ip ep r1 r2 => mkrf ip p r1 r2
+  | R1, mkrf ip ep r1 r2 => mkrf ip ep p r2
+  | R2, mkrf ip ep r1 r2 => mkrf ip ep r1 p
+  end.
+
+Definition rff (rf : RegisterFile) (r: Reg) : Ptr := match r with
+  | IP => ip rf 
+  | EP => ep rf
+  | R1 => r1 rf
+  | R2 => r2 rf
   end.
 
 Inductive State := st {
@@ -42,21 +47,27 @@ Inductive State := st {
   st_h  : Heap
 }.
 
-Definition I (p : Program) : State := st (λ r, 0) p nil nil. 
+Definition I (p : Program) : State := st (mkrf 1 0 0 0) p nil nil. 
 
 Open Scope nat_scope. 
 Inductive read : RO → State → Ptr → Type :=
-  | read_reg : ∀ r s, read (RW (WR r)) s (st_rf s r)
-  | read_mem : ∀ r o rf p s h1 h2 v, 
-    read (RW (WM r o)) (st rf p s (h1++(rf r+o,v)::h2)) v
+  | read_reg : ∀ r s, read (RW (WR r)) s (rff (st_rf s) r)
+  | read_mem : ∀ r o rf p s h v, 
+    lookup (o+rff rf r) h = Some v →
+    read (RW (WM r o)) (st rf p s h) v
   | read_const : ∀ c s, read (RC c) s c.
 
 Inductive write : WO → Word → State → State → Type :=
   | write_reg : ∀ r rf p s h w, 
     write (WR r) w (st rf p s h) (st (upd r w rf) p s h)
-  | write_mem : ∀ r o rf p s h1 h2 v w, 
-    write (WM r o) w (st rf p s (h1++(rf r+o,v)::h2)) 
-                     (st rf p s (h1++(rf r+o,w)::h2)).
+  | write_mem : ∀ r o rf p s h w, 
+    write (WM r o) w (st rf p s h) 
+                     (st rf p s (replace beq_nat (o+rff rf r) w h)).
+
+Fixpoint zeroes (n : nat) (p : Ptr) := match n with
+  | 0 => []
+  | S n => (p, 0)::zeroes n (S p)
+  end.
 
 Inductive step_bb : BasicBlock → State → State → Type := 
   | step_push : ∀ rf p s h ro is v sn,
@@ -68,8 +79,9 @@ Inductive step_bb : BasicBlock → State → State → Type :=
   step_bb is s' sn →
   step_bb (instr (pop wo) is) (st rf p (w::s) h) sn
   | step_new : ∀ rf p s h wo is w s' n sn,
-  write wo w (st rf p s h) s' →
-  (∀ i, i < n → not (In (w+i) (domain h))) →
+  (∀ i, i < n → not (In (i+w) (domain h))) →
+  w > 0 →
+  write wo w (st rf p s (zeroes n w ++ h)) s' →
   step_bb is s' sn → 
   step_bb (instr (new n wo) is) (st rf p s h) sn 
   | step_mov : ∀ s is ro wo s' v sn, 
@@ -80,11 +92,12 @@ Inductive step_bb : BasicBlock → State → State → Type :=
   read ro s 0 →
   write (WR IP) k s s' → 
   step_bb (jump (Some (ro, k)) j) s s'
-  | step_jumpS : ∀ ro k j s s' l, 
-  read ro s (S l) →
+  | step_jumpS : ∀ ro k j s s' l k', 
+  l > 0 →
+  read ro s l →
   read j s k → 
   write (WR IP) k s s' → 
-  step_bb (jump (Some (ro, l)) j) s s'
+  step_bb (jump (Some (ro, k')) j) s s'
   | step_jump : ∀ ro s s' l, 
   read ro s l →
   write (WR IP) l s s' → 
